Start working on some of the necessary infrastructure for a lean LLVM simulator.  Some nontrivial work here that is necessary to unwind type aliases.  We need to ensure that type alias references are well founded, so that all type defintions are sensible and lookups through the map will not result in an infinite chain of following type alias references.

src/ast.lean
@@ -1,12 +1,16 @@
 /- A transliteration of llvm-pretty https://github.com/elliottt/llvm-pretty/blob/master/src/Text/LLVM/AST.hs -/
 import data.bitvec
 import data.rbmap
+import data.string
 
 namespace llvm
 
 -- FIXME
 -- def float : Type 0 := sorry
 -- def double : Type 0 := sorry
+
+def strmap (a:Type) := @rbmap string a string.has_lt'.lt
+def strmap_empty (a:Type) : strmap a := rbmap.from_list []
 
 -- Identifiers -----------------------------------------------------------------
 
@@ -217,8 +221,8 @@ with val_md : Type
   | value : typed value -> val_md
   | ref : nat -> val_md
   | node : list (option val_md) -> val_md
-  | md_loc : debug_loc -> val_md
--- --  | val_md_debug_info (debug_info' lab)
+  | loc : debug_loc -> val_md
+  | debug_info : val_md -- FIXME , just a placeholder for now
 
 with debug_loc : Type
   | debug_loc
@@ -325,7 +329,7 @@ structure global :=
   ( type  : llvm_type                )
   ( value : option value            )
   ( align : option nat              )
-  ( metadata : rbmap string val_md )
+  ( metadata : strmap val_md )
 
 inductive fun_attr
    | align_stack : nat -> fun_attr
@@ -378,15 +382,15 @@ structure basic_block :=
 
 structure define :=
   ( linkage  : option linkage  )
-  ( ret_type  : llvm_type       )
+  ( ret_type : llvm_type       )
   ( name     : symbol         )
   ( args     : list (typed ident)  )
-  ( var_args  : bool           )
+  ( var_args : bool           )
   ( attrs    : list fun_attr   )
   ( sec      : option string  )
   ( gc       : option GC      )
   ( body     : list basic_block)
-  ( metadata : rbmap string val_md)
+  ( metadata : strmap val_md)
   ( comdat   : option string   )
 
 structure global_alias :=
@@ -401,7 +405,7 @@ structure module :=
   ( types      : list type_decl    ) -- ^ top-level type aliases
   ( named_md    : list named_md     )
   ( unnamed_md  : list unnamed_md   )
-  ( comdat     : rbmap string selection_kind)
+  ( comdat     : strmap selection_kind)
   ( globals    : list global   ) -- ^ global value declarations
   ( declares   : list declare  ) -- ^ external function declarations (without definitions)
   ( defines    : list define   ) -- ^ internal function declarations (with definitions)
